\begin{enumerate}
\item On note $A_n=(a_{i,j,n})_{1\leq i,j\leq n}$, $B_n=(b_{i,j,n})_{1\leq i,j\leq n}$, $A_nB_n=(c_{i,j,n})_{1\leq i,j\leq n}$, $A=(\a_{i,j})_{1\leq i,j\leq n}$, $B=(\b_{i,j})_{1\leq i,j\leq n}$ et $AB=(d_{i,j})_{1\leq i,j\leq n}$.\\
On raisonne coefficient par coefficient : pour tout $i,j$, $a_{i,j,n}\tend \a_{i,j}$ et $b_{i,j,n}\tend \b_{i,j}$.\\
Alors pour tout $i,j$, $c_{i,j,n}=\dsum_{k=1}^p a_{i,k,n}b_{k,j,n}\tend \dsum_{k=1}^p \a_{i,k}\b_{k,j}=d_{i,j}$, donc $A_nB_n\tend AB$.
\item
$(A^n)^2\tend P^2$ mais aussi $(A^n)^2=A^{2n}\tend P$ donc $P=P^2$.
\end{enumerate}
